parallel preimage

Matroid/Constructions/ParallelExt.lean
@@ -4,18 +4,17 @@ import Matroid.Constructions.Basic
 
 open Set Function
 
-variable {α β : Type _}
- 
+variable {α β : Type _} {f : α → β} {s : Set α}
+
 lemma Function.invFunOn_injOn_image_preimage [_root_.Nonempty α] (f : α → β) (S : Set α) : 
     InjOn f ((invFunOn f S) '' (f '' S)) := by
   rintro _ ⟨_,⟨x,hx, rfl⟩,rfl⟩ _ ⟨_,⟨y,hy,rfl⟩,rfl⟩ h
   rw [invFunOn_eq (f := f) ⟨x, hx, rfl⟩, invFunOn_eq (f := f) ⟨y,hy,rfl⟩] at h
   rw [h]
-  
-
 
 lemma Set.InjOn.exists_injOn_superset {f : α → β} {s t : Set α} (hinj : InjOn f s) (hst : s ⊆ t) : 
     ∃ r, s ⊆ r ∧ r ⊆ t ∧ InjOn f r ∧ f '' r = f '' t := by 
+  
   obtain (hα | hα) := isEmpty_or_nonempty α
   · exact ⟨∅, by simp [eq_empty_of_isEmpty]⟩ 
   set d := t ∩ (f ⁻¹' (f '' t \ f '' s)) with hd
@@ -53,206 +52,63 @@ lemma Set.InjOn.exists_injOn_superset {f : α → β} {s t : Set α} (hinj : Inj
   rintro _ ⟨_, ⟨x, hx, rfl⟩, rfl⟩
   exact mem_of_mem_of_subset (invFunOn_apply_mem (f := f) hx) (inter_subset_left _ _)
 
-
 lemma Set.InjOn.exists_injOn_superset_image {f : α → β} {s s' : Set α} {t : Set β} 
     (hss' : s ⊆ s') (hinj : InjOn f s) (hst : f '' s ⊆ t) (ht : t ⊆ f '' s') : 
     ∃ r, s ⊆ r ∧ r ⊆ s' ∧ InjOn f r ∧ f '' r = t := by 
-  obtain (hα | hα) := isEmpty_or_nonempty α
-  · simp only [eq_empty_of_isEmpty, injOn_empty, image_empty, empty_subset, true_and, 
-      exists_const, subset_empty_iff, eq_comm (a := t)] at *
-    assumption 
-  set d := s' ∩ f ⁻¹' (t \ f '' s) with hd
-  set g := f.invFunOn d with hg
-  have hds' : d ⊆ s' \ s
-  · rw [hd, preimage_diff, subset_diff, and_iff_right (inter_subset_left _ _), 
-      disjoint_iff_forall_ne]
-    rintro a ⟨has', ha, ha'⟩ b hb rfl 
-    exact ha' (mem_image_of_mem _ hb)
-
-  refine ⟨s ∪ (g '' (f '' d)), subset_union_left _ _, union_subset hss' ?_, ?_, ?_⟩
-  · refine (invFunOn_image_image_subset _ _).trans (subset_diff.1 hds').1
-  · rw [injOn_union, and_iff_right hinj, and_iff_right (invFunOn_injOn_image_preimage _ _)]
-    · rintro x hxs _ ⟨_, ⟨y, hy, rfl⟩, rfl⟩ he
-      rw [invFunOn_apply_eq (f := f) hy] at he
-      apply hy.2.2
-      rw [←he]
-      exact mem_image_of_mem f hxs
-    exact disjoint_of_subset_right (invFunOn_image_image_subset _ _) (subset_diff.1 hds').2.symm
-  
-  rw [image_union, subset_antisymm_iff, union_subset_iff, and_iff_right hst, and_iff_left]
-  · rintro _ ⟨_, ⟨_, ⟨ x, hx, rfl⟩, rfl⟩, rfl⟩  
-    refine mem_of_mem_of_subset (mem_image_of_mem f (invFunOn_apply_mem (f := f) hx)) ?_
-    rintro _ ⟨y, ⟨-, hy⟩, rfl⟩  
-    exact hy.1 
-  
-  · sorry 
-  
-  -- refine ht.trans ?_
-  -- rintro _ ⟨x, hx, rfl⟩ 
-  -- by_cases h : f x ∈ f '' s
-  -- · left; assumption
-  -- rw [mem_union]; right
-  -- refine ⟨g (f x), ?_, ?_⟩ 
-  -- · rw [invFunOn_]
-
-
-    
-  -- obtain ⟨r, hsr, h', hi, hr⟩ := hinj.exists_injOn_superset (image_subset_iff.1 hst)
-  -- refine ⟨r, hsr, ?_, hi, ?_⟩ 
-  -- refine ⟨r, hsr, hi, by rwa [hr, image_preimage_eq_iff]⟩  
-  
-  
-
-  
-
+  rw [image_subset_iff] at hst
+  obtain ⟨r, hsr, hrs', hinj, heq⟩ := hinj.exists_injOn_superset (subset_inter hss' hst)
+  rw [subset_inter_iff] at hrs'
+  refine ⟨r, hsr, hrs'.1, hinj, ?_⟩ 
+  rw [heq, subset_antisymm_iff, image_subset_iff, and_iff_right (inter_subset_right _ _)]
+  intro x hxt
+  obtain ⟨y, hy, rfl⟩ := ht hxt 
+  exact ⟨y, ⟨hy, hxt⟩, rfl⟩  
 namespace Matroid
   
+/-- Given a `Matroid` `M` on `β` and a function `f : α → β`, this is the matroid on `α` 
+  obtained by replacing each `x ∈ M.E` by the fiber `f ⁻¹' {x}` of pairwise parallel elements -/
 def parallel_preimage (M : Matroid β) (E : Set α) (f : α → β) : Matroid α := matroid_of_indep
-  E 
-  ( fun I ↦ M.Indep (f '' I) ∧ InjOn f I ∧ I ⊆ E )
-  ( by simp )
+  E ( fun I ↦ M.Indep (f '' I) ∧ InjOn f I ∧ I ⊆ E ) ( by simp )
   ( fun I J ⟨h, h', hE⟩ hIJ ↦ ⟨h.subset (image_subset _ hIJ), InjOn.mono hIJ h', hIJ.trans hE⟩ )
   ( by
     rintro I J ⟨hI, hIinj, hIE⟩ hImax hJmax
 
-    have hI1 : ¬M.Base (f '' I)
-    · refine fun hI' ↦ hImax ⟨⟨hI, hIinj, hIE⟩, fun B ⟨hB, hBinj, hBE⟩ (hB' : _ ⊆ _) x hxB ↦ 
-        hBinj.mem_of_mem_image hB' hxB ?_⟩
-      rw [hI'.eq_of_subset_indep hB (image_subset _ hB')]
-      exact mem_image_of_mem _ hxB
-    simp only [mem_maximals_iff, mem_setOf_eq, and_imp] at hJmax hImax
-    simp only [not_and, not_forall, exists_prop, exists_and_left, and_imp, hI, hIinj, hIE, 
-      forall_true_left] at hImax 
+    simp only [mem_maximals_iff, mem_setOf_eq, and_imp, hI, hIinj, hIE, and_self, true_and, 
+      not_forall, exists_prop, exists_and_left] at hJmax hImax 
+    
+    obtain ⟨B', hB', hB'inj, hB'E, hIB', hne⟩ := hImax 
     obtain ⟨⟨hJ, hJinj, hJE⟩, hJmax⟩ := hJmax
+  
+    have hi : (M ↾ f '' E).Indep (f '' I) := hI.indep_restrict_of_subset (image_subset f hIE)
+
+    have h1 : ¬(M ↾ f '' E).Base (f '' I)
+    · exact fun hB ↦ hne <| (hB'inj.image_eq_image_iff_of_subset hIB' Subset.rfl).1
+        (hB.eq_of_subset_indep (hB'.indep_restrict_of_subset (image_subset _ hB'E))
+        (image_subset _ hIB'))
+      
+    have h2 : (M ↾ f '' E).Base (f '' J)
+    · apply (hJ.indep_restrict_of_subset (image_subset _ hJE)).base_of_maximal
+      simp_rw [restrict_indep_iff]
+      rintro K' ⟨hK', hK'E⟩ hJK'
+      obtain ⟨K, hJK, hKE, hKinj, rfl⟩ := hJinj.exists_injOn_superset_image hJE hJK' hK'E
+      rw [hJmax hK' hKinj hKE]
+      rwa [←hKinj.image_subset_image_iff_of_subset hJK Subset.rfl]
     
-    set M' := (M ↾ f '' E) with hM'
-
-    have hi : M'.Indep (f '' I)
-    · exact hI.indep_restrict_of_subset (image_subset f hIE)
-
-    have h1 : ¬M'.Base (f '' I)
-    · sorry 
-    
-    have h2 : M'.Base (f '' J)
-    · sorry
-
-
     obtain ⟨_, ⟨⟨e, heJ, rfl⟩, heI⟩, hi⟩ := hi.exists_insert_of_not_base h1 h2
     have heI' : e ∉ I := fun heI' ↦ heI (mem_image_of_mem f heI')
     refine' ⟨e, ⟨heJ, heI'⟩, _, _, insert_subset (hJE heJ) hIE⟩ 
     · rw [image_insert_eq]
       exact hi.of_restrict
-    rw [injOn_insert heI', and_iff_right hIinj]
-    assumption 
-
-
-    -- have h1 : ¬M.Basis (f '' I) (f '' E ∩ M.E) 
-    -- · obtain ⟨I', hI', hI'inj, hI'E, hII', hne⟩ := hImax
-    --   refine fun hb ↦ hne <| hII'.antisymm <| fun x hx ↦ ?_
-    --   apply hI'inj.mem_of_mem_image hII' hx
-    --   rw [hb.eq_of_subset_indep hI' (image_subset _ hII') 
-    --     (subset_inter (image_subset _ hI'E) hI'.subset_ground) ]
-    --   exact mem_image_of_mem _ hx
-      
-    -- have h2 : M.Basis (f '' J) (f '' E ∩ M.E)
-    -- · refine hJ.basis_of_maximal_subset (subset_inter (image_subset _ hJE) (hJ.subset_ground)) 
-    --     (fun K hK hJK hKE ↦ ?_) (inter_subset_right _ _)
-    --   have' := hJinj.exists_injOn_superset_image 
-    --   -- rw [subset_inter_iff] at hKE
-      -- have := image_subset_iff.1 hJK
-      -- have := hJinj.exists_injOn_superset hJE
-      
-      
-    -- obtain ⟨K', hJK', hKinj', rfl⟩ := hJinj.exists_injOn_superset_image hJK ?_
-      
-        -- (subset_inter (image_subset_iff.1 hJK) hJE)
-      
-      -- rw [hJmax hK hKinj' _ hJK']
-      -- · rw [h_eq]
-      --   intro x hxk
-
-      --   exact hKE.trans ((inter_subset_left _ _).trans (image_subset_range _ _))
-      
-        
-      
-      -- have := hJmax (y := (f ⁻¹' K ∩ E)) 
-      --   (hK.subset (subset_trans (image_subset _ (inter_subset_left _ _)) 
-      --     (image_preimage_subset f _)))
-
-      -- have hA : ∃ A, J ⊆ A ∧ A ⊆ E ∧ InjOn f A ∧ f '' A = K
-      -- · set D := K \ f '' J with hD
-      --   set S := f ⁻¹' D ∩ E with hS 
-      --   set g : β → α := Function.invFunOn f S with hg
-        
-      --   have hdj : Disjoint J (g '' (f '' S))
-      --   · refine' disjoint_of_subset_right (invFunOn_image_image_subset ?_ ?_) ?_ 
-      --     simp_rw [hS, hD, disjoint_iff_forall_ne, mem_inter_iff, mem_preimage]
-      --     rintro a haJ b ⟨⟨-,hb⟩,-⟩ rfl 
-      --     exact hb (mem_image_of_mem _ haJ)
-
-      --   refine ⟨J ∪ g '' (f '' S), subset_union_left _ _, union_subset hJE ?_, ?_, ?_⟩ 
-      --   · exact (Function.invFunOn_image_image_subset f _).trans (inter_subset_right _ _)
-      --   · rw [injOn_union, and_iff_right hJinj, and_iff_right (invFunOn_injOn_image_preimage _ _)]
-      --     · rintro x hxJ _ ⟨_, ⟨⟨y, hy', rfl⟩, hy, rfl⟩⟩ he 
-      --       have hmem := mem_image_of_mem f <| invFunOn_mem (f := f) (s := S) ⟨y, hy', rfl⟩
-      --       rw [←hg, ←he, hS, hD] at hmem
-      --       obtain ⟨a, ha, he⟩:= hmem
-      --       rw [mem_inter_iff, mem_preimage, he] at ha
-      --       exact ha.1.2 (mem_image_of_mem _ hxJ)
-      --     exact hdj
-        
-          
-          
-
-          
-          
-
-      --     -- union_subset hJE (inter_subset_right _ _), ?_, ?_⟩ 
-      --   -- · rw [injOn_union, and_iff_right hJinj]
-        
-   
-      
-      
-      
-
-
-    
-
-    -- obtain ⟨_, ⟨⟨x,hx,rfl⟩,h'⟩, he'⟩ := hI.exists_insert_of_not_basis (image_subset f hIE) h1 h2
-    -- refine' ⟨x, ⟨hx, fun hxI ↦ h' (mem_image_of_mem f hxI)⟩, _, _, _⟩ 
-    -- · rwa [image_insert_eq]
-    -- · rw [injOn_insert (fun hxI ↦ h' (mem_image_of_mem f hxI))]
-    --   exact ⟨hIinj, h'⟩ 
-
-    -- exact insert_subset (hJE hx) hIE
-
-
-
-
-
-    -- have hB1 : M.Base (f '' J)
-    -- · simp only [mem_maximals_iff, mem_setOf_eq, and_imp] at hJmax 
-    --   refine hJmax.1.1.base_of_maximal (fun K hK hss ↦ ?_)
-    --   have := hJmax.2 (y := (f ⁻¹' K) ∩ E) (hK.subset ?_)
-
-    --   rw [hJmax.2 (y := (f ⁻¹' K) ∩ E)]
-      
-      
-    
-
-    --
-    -- simp [mem_maximals_iff, iff_true_intro hI, iff_true_intro hIinj, iff_true_intro hIE] at hImax
-    
-  )
+    rwa [injOn_insert heI', and_iff_right hIinj] )
   ( by
     rintro X hXE I ⟨hI, hIinj, hIE⟩ hIX
-    set M' := M ↾ (f '' E) with hM'
+    set M' := M ↾ (f '' E)
     have hI' : M'.Indep (f '' I)
     · exact restrict_indep_iff.2 ⟨hI, image_subset f hIE⟩ 
     obtain ⟨J, hJX, hIJ⟩ := hI'.subset_basis_of_subset (image_subset f hIX) (image_subset f hXE)
     obtain ⟨J, hIJ', hJX', hJinj, rfl⟩ := hIinj.exists_injOn_superset_image hIX hIJ hJX.subset    
     refine ⟨J, ⟨⟨hJX.indep.of_restrict, hJinj, hJX'.trans hXE⟩, hIJ', hJX'⟩, ?_⟩ 
-    rintro B ⟨⟨hB, hBinj, hBE⟩,  hIB, hBX⟩ (hJB : J ⊆ B) b hb
+    rintro B ⟨⟨hB, hBinj, hBE⟩, -, hBX⟩ (hJB : J ⊆ B) b hb
     have hB' : M'.Indep (f '' B)
     · refine restrict_indep_iff.2 ⟨hB, image_subset f hBE⟩ 
     have hb' := mem_image_of_mem f hb
@@ -260,11 +116,9 @@ def parallel_preimage (M : Matroid β) (E : Set α) (f : α → β) : Matroid α
     exact hBinj.mem_of_mem_image hJB hb hb' )
   ( fun I h ↦ h.2.2 )
 
-
-
 @[simp] theorem parallel_preimage_indep_iff {M : Matroid β} {E : Set α} {f : α → β} {I : Set α} : 
     (M.parallel_preimage E f).Indep I ↔ (M.Indep (f '' I) ∧ InjOn f I ∧ I ⊆ E) := by 
-  sorry 
+  simp [parallel_preimage]
 
 @[simp] theorem parallel_preimage_ground_eq {M : Matroid β} {E : Set α} {f : α → β} : 
     (M.parallel_preimage E f).E = E := rfl 
